cbvlcm: Heaps: up to lookup def (done)

hol_cbvlcm2/HeapsScript.sml
@@ -8,7 +8,39 @@ val _ = new_theory "Heaps";
            Heaps
    --------------------- *)
 
+Type Heap = ``:(('a # num) # num) list``;
+Type HA = ``:num``;
+Type HC = ``:'a # HA``;
+Type HE = ``:(('a HC) # HA) option``;
 
+Datatype:
+  heap =
+    <|
+      get : 'a Heap -> HA -> ('a HE) option;
+      put : 'a Heap -> 'a HC -> HA -> ('a Heap) # HA;
+    |>
+End
+
+Definition extended:
+  extended H H' hImpl =
+    ∀a. hImpl.get H a ≠ NONE ⇒ hImpl.get H a = hImpl.get H' a
+End
+
+Definition HR1:
+  HR1 hImpl =
+    ∀H g a H' b.
+      hImpl.put H g a = (H', b) ⇒ hImpl.get H' b = SOME (SOME (g,a))
+End
+
+Definition HR2:
+  HR2 hImpl =
+    ∀H g a H' b.
+      hImpl.put H g a = (H', b) ⇒ extended H H' hImpl
+End
+
+Definition HR:
+  HR hImpl = (HR1 hImpl ∧ HR2 hImpl)
+End
 
 (*
 Class heap PA :=
@@ -25,70 +57,115 @@ Class heap PA :=
   }.
 
 Coercion get : Heap >-> Funclass.
+*)
 
+(*
 Section heap.
   Variable codeImpl : code.
   Variable C : Code.
   Variable heapImpl : heap PA.
   Implicit Type H : Heap.
+*)
 
-  Reserved Notation "a ≫E_ H E" (at level 70, H at level 0, format "a '≫E_' H E").
+(* Reserved Notation "a ≫E_ H E" (at level 70, H at level 0, format "a '≫E_' H E"). *)
+(* "a ≫E_ H E" := (representsEnv H a E). *)
+(* HA -> list Clo -> Prop *)
+Inductive representsEnv:
+[~Nil:]
+  (∀hImpl C H a. hImpl.get H a = SOME NONE ⇒ representsEnv hImpl C H a []) ∧
+[~Cons:]
+  (∀hImpl C H a b c p P F E.
+         hImpl.get H a = SOME (SOME ((p, b), c)) ∧
+         representsPro C p P ∧
+         representsEnv hImpl C H b F ∧
+         representsEnv hImpl C H c E ⇒
+         representsEnv hImpl C H a ((closC P F)::E)
+  )
+End
 
-  Inductive representsEnv H : HA -> list Clo -> Prop :=
-  | representsEnvNil a:
-      H a = Some None ->
-      a ≫E_H []
-  | representsEnvCons a b c p P F E:
-      H a = Some(Some ((p,b),c)) ->
-      p ≫p_C P ->
-      b ≫E_H F ->
-      c ≫E_H E ->
-      a ≫E_H (P/F)::E
-  where "a ≫E_ H E" := (representsEnv H a E).
+Theorem representsEnv_functional:
+  ∀hImpl C H. functional (representsEnv hImpl C H)
+Proof
+  simp[functional] >>
+  Induct_on `representsEnv` >> rw[] (* 2 *)
+  >- (fs[Once representsEnv_cases] >> fs[])
+  >> pop_assum mp_tac >> rw[Once representsEnv_cases] >>
+  metis_tac[representsPro_functional, functional]
+QED
 
-  Hint Constructors representsEnv.
+Theorem representsEnv_extend:
+  ∀C hImpl H H' a E.
+    extended H H' hImpl ⇒
+    representsEnv hImpl C H a E ⇒
+    representsEnv hImpl C H' a E
+Proof
+  Induct_on `representsEnv` >> rw[]
+  >- (fs[extended] >>
+      `hImpl.get H a ≠ NONE` by fs[] >>
+      first_x_assum drule >> rw[] >>
+      rw[Once representsEnv_cases])
+  >> rw[Once representsEnv_cases] >>
+  qexistsl_tac [`a'`, `a''`, `p`] >> rw[] >>
+  fs[extended] >>
+  `hImpl.get H a ≠ NONE` by fs[] >>
+  first_x_assum drule >> rw[]
+QED
 
-  Lemma representsEnv_functional H:
-  functional (representsEnv H).
-  Proof.
-    intros a E E' H1. induction H1 in E'|-*; inversion 1;try congruence;repeat f_equal. all:rewrite H0 in H3;inv H3. all:now try eapply representsPro_functional;eauto.
-  Qed.
-  Lemma representsEnv_extend H H' a E :
-    extended H H' -> a ≫E_H E -> a ≫E_H' E.
-  Proof.
-    intros ext. induction 1 as [? eq|? ? ? ? ? ? ? eq].
-    -econstructor. erewrite ext in eq. eauto. congruence.
-    -econstructor. 2-4:now eauto.
-     erewrite ext in eq. eauto. congruence.
-  Qed.
-  Reserved Notation "g ≫C_ H e" (at level 70,H at level 0, format "g '≫C_' H e").
+(*  Reserved Notation "g ≫C_ H e" (at level 70,H at level 0, format "g '≫C_' H e"). *)
+Inductive representsClos:
+[~C:]
+  (∀hImpl p a P E.
+    representsPro C p P ∧
+    representsEnv hImpl C H a E ⇒
+    representsClos hImpl C H (p,a) (closC P E))
+End
 
+(*
   Inductive representsClos H : HC -> Clo -> Prop :=
     representsClos_C p a P E : p ≫p_C P -> a ≫E_H E -> (p,a) ≫C_H P/E
   where "g ≫C_ H e" := (representsClos H g e).
   Hint Constructors representsClos.
 
   Notation "(≫C( H ) )" := (representsClos H) (at level 0, format "'(≫C(' H ')' ')'").
-  (* workaround to prefere "x ≻ y" over "(≻) x y"*) Notation "g ≫C_ H e" := 0.
+  Notation "g ≫C_ H e" := 0.
   Notation "g ≫C_ H e" := (representsClos H g e).
+*)
 
-  Lemma representsClos_extend H H' g e :
-    extended H H' -> g ≫C_H e -> g ≫C_H' e.
-  Proof.
-    intros ext. inversion 1. all:eauto using representsEnv_extend.
-  Qed.
+Theorem representsClos_extend:
+  ∀H H' g e hImpl C.
+    extended H H' hImpl ⇒
+    representsClos hImpl C H g e ⇒
+    representsClos hImpl C H' g e
+Proof
+  rw[] >> fs[Once representsClos_cases] >>
+  metis_tac[representsEnv_extend]
+QED
 
-  Fixpoint lookup H a n : option HC:=
-    match H a with
-      Some (Some (g,a')) =>
-      match n with
-        0 => Some g
-      | S n=> lookup H a' n
-      end
-    | _ => None
-    end.
-  Notation "H .[ a , n ]" := (lookup H a n) (at level 1, format "H '.[' a ',' n ]").
+(* Notation "H .[ a , n ]" := (lookup H a n) (at level 1, format "H '.[' a ',' n ]"). *)
+Definition lookup:
+  lookup hImpl H a n =
+    case (hImpl.get H a) of
+      SOME (SOME (g, a')) =>
+        (case n of
+          0 => SOME g
+        | SUC n => lookup hImpl H a' n)
+      | _ => NONE
+End
 
+Theorem nth_error_unlinedEnv:
+  ∀hImpl C H a E n e.
+    representsEnv hImpl C H a E ⇒
+    nth_error n E = SOME e ⇒
+    (∃g. lookup hImpl H a n = SOME g ∧
+         representsClos hImpl C H g e)
+Proof
+  Induct_on `n` >> rw[]
+  >- cheat
+  >> cheat
+QED
+
+
+(*
   Lemma nth_error_unlinedEnv H a E n e :
     a ≫E_H E -> E.[n] = Some e -> exists g, H.[a,n] = Some g /\ g ≫C_H e.
   Proof.
@@ -129,5 +206,19 @@ Proof.
    rewrite nth_error_app1;eauto using nth_error_Some_lt. now rewrite eq.
 Defined
 *)
+
+Definition heapImpl:
+  heapImpl =
+    <|
+      put := (λH g a. (H++[(g,a)], SUC (LENGTH H)));
+      get := (λH a. case a of
+                     | 0 => SOME NONE
+                     | SUC a =>
+                       (case nth_error a H of
+                        | SOME (g,b) => SOME (SOME (g,b))
+                        | NONE => NONE)
+             )
+    |>
+End
 
 val _ = export_theory ()
